restore original popMax

Batteries/Data/BinaryHeap/Basic.lean
@@ -102,29 +102,24 @@ def insert [Ord α] (self : BinaryHeap α) (x : α) : BinaryHeap α where
 /-- `O(1)`. Get the maximum element in a `BinaryHeap`. -/
 def max (self : BinaryHeap α) : Option α := self.1[0]?
 
--- Helper function that performs popMax on the underlying vector
--- Exists because it made verification somewhat easier
-private def popMaxVec [Ord α] (v : Vector α sz) : Vector α (sz - 1)  :=
-  if h0 : sz = 0 then
-    (by omega : sz = sz - 1 ) ▸ v
-  else
-    have hs : sz - 1 < sz := by omega
-    have h0 : 0 < sz := Nat.zero_lt_of_ne_zero h0
-    let v := v.swap 0 (sz - 1) |>.pop
-    if h : 0 < sz - 1 then
-      heapifyDown v ⟨0, h⟩
-    else
-      v
-
-/-- `O(log n)`. Remove the maximum element from a `BinaryHeap`.
-Call `max` first to actually retrieve the maximum element. -/
-@[inline]
+/-- `O(log n)`. Remove the maximum element from a `BinaryHeap`.-/
+@[expose]
 def popMax [Ord α] (self : BinaryHeap α) : BinaryHeap α :=
-  ⟨popMaxVec self.vector |>.toArray⟩
+  if h0 : self.size = 0 then self else
+    have hs : self.size - 1 < self.size := Nat.pred_lt h0
+    have h0 : 0 < self.size := Nat.zero_lt_of_ne_zero h0
+    let v := self.vector.swap _ _ h0 hs |>.pop
+    if h : 0 < self.size - 1 then
+      ⟨heapifyDown v ⟨0, h⟩ |>.toArray⟩
+    else
+      ⟨v.toArray⟩
 
 @[simp] theorem size_popMax [Ord α] (self : BinaryHeap α) :
     self.popMax.size = self.size - 1 := by
-  simp [popMax, size]
+  simp only [popMax, size]
+  split
+  · simp +arith [*]
+  · split <;> simp +arith
 
 /-- `O(log n)`. Return and remove the maximum element from a `BinaryHeap`. -/
 def extractMax [Ord α] (self : BinaryHeap α) : Option α × BinaryHeap α :=
